# Lecture 27 - Notes  

### July 8, 2015  

### Mathematical Induction

Let $P(n)$ be a statement whose truth-value is dependant upon the variable $n$. Then $P(n)$ is true for all $n \ge n_0$ if both of the following hold,

1. $P(n)$ is true for $n = n_0$ (base)
2. If $P(k)$ is true for $K \ge n_0$, then $P(k+1)$ is also true (inductive step)

#### Example

Prove that for all $n \ge 1$,

$$\begin{aligned}
    \frac{1}{1\cdot2} + \frac{1}{2\cdot3} + \frac{1}{3\cdot4} + ... + \frac{1}{n(n+1)} &= \frac{n}{n+1} \newline
\end{aligned}$$

##### Solution

Let $P(n)$ be the statement,

$$\begin{aligned}
    \sum_{i=1}^{n} \frac{1}{i(i+1)} = \frac{n}{n+1}
\end{aligned}$$

where $n \in \mathbb N$, $n \ge 1$.

###### Base

Consider the base case $P(1)$ where $n = 1$, on the left hand side,

$$\begin{aligned}
    \sum_{i=1}^{n} \frac{1}{i(i+1)} &= \sum_{i=1}^{1} \frac{1}{i(i+1)} \newline
    &= \frac{1}{1(1+1)} \newline
    &= \frac{1}{2}
\end{aligned}$$

on the right hand side,

$$\begin{aligned}
    \frac{n}{n+1} &= \frac{1}{1+1} \newline
    &= \frac{1}{2} \newline
\end{aligned}$$

since the left hand side equals the right hand side, $P(1)$ holds.

###### Inductive Hypothesis

Suppose $P(k)$ is true for $k \ge 1$,

$$\begin{aligned}
    \sum_{i=1}^{k} \frac{1}{i(i+1)} = \frac{k}{k+1}
\end{aligned}$$

###### Inductive Step

Consider $P(k+1)$, on the left hand side,

$$\begin{aligned}
    \sum_{i=1}^{k+1} \frac{1}{i(i+1)} &= \frac{1}{1\cdot2} + \frac{1}{2\cdot3} + ... + \frac{1}{k\cdot(k+1)} + \frac{1}{(k+1)\cdot((k+1)+1)} \newline  
    &= \frac{1}{1\cdot2} + \frac{1}{2\cdot3} + ... + \frac{1}{k\cdot(k+1)} + \frac{1}{(k+1)\cdot(k+2)} \newline
    &= \left(\sum_{i=1}^{k} \frac{1}{i(i+1)} \right) + \frac{1}{(k+1)\cdot(k+2)} \newline
    &= \frac{k}{k+1} + \frac{1}{(k+1)\cdot(k+2)} \newline
    &= \frac{k(k+2)}{(k+1)\cdot(k+2)} + \frac{1}{(k+1)\cdot(k+2)} \newline
    &= \frac{k(k+2) + 1}{(k+1)\cdot(k+2)} \newline
    &= \frac{k^2 + 2k + 1}{(k+1)\cdot(k+2)} \newline
    &= \frac{(k + 1)\cdot(k+1)}{(k+1)\cdot(k+2)} \newline
    &= \frac{k+1}{k+2} \newline
\end{aligned}$$

 on the right hand side,
 
 $$\begin{aligned}
    \frac{k+1}{(k+1) + 1} = \frac{k+1}{k+2}
\end{aligned}$$

since the left hand side is equal to the right hand side, $P(k+1)$ holds. Therefore, by induction, $P(n)$ holds for all $n \in \mathbb N$ where $n \ge 1$.

#### Example

Prove that for $n \in \mathbb N$ where $n \ge 5$, $4n \le 2^n$.

##### Solution

Let $P(n)$ be the statement,

$$
    4n \le 2^n
$$

for all $n \in \mathbb n$ where $n \ge 5$.

###### Base

Consider $P(5)$, on the left hand side,

$$\begin{aligned}
    4n &= 4 \cdot 5 \newline
    &= 20 \newline
\end{aligned}$$

on the right hand side,

$$\begin{aligned}
    2^n &= 2^5 \newline
    &= 32 \newline
\end{aligned}$$

since the left hand side is less than the right hand side, $P(5)$ holds.

###### Inductive Hypothesis

Suppose $P(k)$ is true for $k \ge 5$, i.e.,

$$\begin{aligned}
    4k \le 2^k
\end{aligned}$$

###### Inductive Step

Consider $P(k+1)$, on the left hand side,

$$\begin{aligned}
    4(k+1) &= 4k + 4 \newline
    &\le 2^k + 4 \newline
    &= 2^k + 2^2 \newline
    &\le 2^k + 2^k \newline
    &= 2\cdot2^k \newline
    &= 2^{k+1} \newline
\end{aligned}$$

on the right hand side,

$$\begin{aligned}
    2^{k+1}
\end{aligned}$$

since the left hand side is less than or equal to the right hand side, if $P(k)$ is true then $P(k+1)$ holds for all $k \in \mathbb N$ where $k \ge 5$. Therefore, by induction, $P(n)$ is true for all $n \in \mathbb N$.



 


