# Lecture 16 - Notes  

### June 10, 2015  

## Section 3.2 Continued

#### Example

$$
\begin{aligned}
    A &= \{ 1,2,3,4 \} \newline
    B &= \{ w,x,y,z \} \newline
    C &= \{ a,b,c \} \newline
\end{aligned}
$$

$$
\begin{aligned}
    f&: A \mapsto B &\text{ where } f = \{ (1,w),(2,z),(3,x),(4,w) \} \newline
    g&: B \mapsto C &\text{ where } g = \{ (w,a),(x,c),(y,b),(z,a) \} \newline
\end{aligned}
$$

##### Solution

Potatoes.

$$
\begin{aligned}
    g \circ f = \{ (1,a),(2,a),(3,c)(4,a) \}
\end{aligned}
$$
$$
\begin{aligned}
    f \circ g = \text{ not a function}
\end{aligned}
$$
$$
\begin{aligned}
    (g \circ f)^{-1} = \text{ not a function}
\end{aligned}
$$

#### Notation

* $f^2 = f \circ f$
* $f^n = f \circ f \circ ... \circ f$

#### Proposition

if $f: A \mapsto B$ and $g: B \mapsto C$ are bijections, then $g \circ f$ is also a bijection.

##### Proof

_(one-to-one)_ Supposed that $g \circ f(x_1) = g \circ f(x_2)$, for some $x_1, x_2 \in A$, or in another notation,

$$%Aligned
\begin{aligned}
    g(f(x_1)) = g(f(x_2))
\end{aligned}
$$

Since $g$ is one-to-one and $g(f(x_1)) = g(f(x_2))$,

$$ %Aligned
\begin{aligned}
    f(x_1) = f(x_2)
\end{aligned}
$$

then since, $f$ is one-to-one and $f(x_1) = f(x_2)$,

$$ %Aligned
\begin{aligned}
    x_1 = x_2
\end{aligned}
$$

So $g \circ f$ is one-to-one.

_(onto)_ Consider $c \in C$, since $g$ is onto,

$$ %Aligned
\begin{aligned}
    \exists b \in B \text{ such that } g(b) = c
\end{aligned}
$$

and since $f$ is onto,

$$ %Aligned
\begin{aligned}
    \exists a \in A \text{ such that } f(a) = b
\end{aligned}
$$

$$ %Aligned
\begin{aligned}
    \therefore g(b) = g(f(a)) = c
\end{aligned}
$$

and $g \circ f$ is onto.

Since $g \circ f$ is one-to-one and onto it is a bijection.

### Inverses and Identities

#### Proposition

Given two functions $f: A \mapsto B$ and $g: B \mapsto A$ are inverses if and only is their compositions are identities.

$$ %Aligned
\begin{aligned}
    g \circ f &= i_A \newline
    f \circ g &= i_B \newline
\end{aligned}
$$

#### Example

$$ %Aligned
\begin{aligned}
    f(x) &= \frac{2x}{x-1} \newline
    g(x) &= \frac{x}{x-2} \newline
\end{aligned}
$$

##### Solution

$$ %Aligned
\begin{aligned}
    g \circ f &= \frac{\frac{2x}{x-1}}{\frac{2x}{x-1}-2} \newline
    &= \frac{\frac{2x}{x-1}}{\frac{2x}{x-1}-2} \cdot \frac{x-1}{x-1} \newline
    &= \frac{2x}{2x-2x+2} \newline
    &= \frac{2x}{2} \newline
    &= x \newline
\end{aligned}
$$

$$ %Aligned
\begin{aligned}
    f \circ g &= \frac{2\left( \frac{x}{x-2} \right)}{\left( \frac{x}{x-2} \right)-1} \newline
    &= \frac{2\left( \frac{x}{x-2} \right)}{\left( \frac{x}{x-2} \right)-1} \cdot \frac{x-2}{x-2} \newline
    &= \frac{2x}{2} \newline
    &= x \newline
\end{aligned}
$$

## Section 3.3 - One-to-one correspondences and the Cardinality of a Set

### Cardinality

_definition_: The __cardinality__ of set $A$, denoted $|A|$, is the number of elements in set $A$.

#### Example

$$ %Aligned
\begin{aligned}
    A &= \{ a,b,c \} \newline
    |A| &= 3 \newline
\end{aligned}
$$

### One-to-one Correspondences

_definition_: A function $f: A \mapsto B$ that is a bijection is also a __one-to-one correspondence__. We say $\exists$ a one-to-one correspondence between $A$ and $B$.

#### Fact

$$ %Aligned
\begin{aligned}
    |A| = |B| \iff \exists ~f:A \mapsto B \text{ that is a bijection.}
\end{aligned}
$$

#### Claim

$$ %Aligned
\begin{aligned}
    |(0,1)| = |(2,5)|
\end{aligned}
$$

##### Proof

Consider $f: (0,1) \mapsto (2,5)$, where,

$$ %Aligned
\begin{aligned}
    f = 2x + 3 \newline
\end{aligned}
$$

_(one-to-one)_ Supposed $f(x_1) = f(x_2)$,

$$ %Aligned
\begin{aligned}
    3x_1 + 2 &= 3x_2 + 2 \newline
    3x_1 &= 3x_2 \newline
    x_1 &= x_2 \newline
\end{aligned}
$$

_(onto)_ Let $y \in (2,5)$, if $f(x) = y$,

$$ %Aligned
\begin{aligned}
    3x + 2 &= y \newline
    3x &= y - 2 \newline
    x &= \frac{y-2}{3} \newline
\end{aligned}
$$

$$ %Aligned
\begin{aligned}
    \therefore f \text{ is a bijection.}
\end{aligned}
$$
