# Lecture 4 - Notes  

### May 12, 2015  

## Section 1.2 Continued

### Using Laws of Logic to prove logical equivalence


#### Example

Show $ p \leftrightarrow q \iff (p \wedge q) \vee (\neg p \wedge \neg q) $.

##### Solution

Proof:

We know,

$$ p \leftrightarrow q \iff (p \to q) \vee (q \to p) $$

and,

$$ p \leftrightarrow q \iff (\neg p \vee q) \wedge (\neg q \vee p) $$

Using distribution twice,

$$ p \leftrightarrow q \iff [(\neg p \vee q) \wedge \neg q] \vee [(\neg p \vee q) \wedge p] $$

$$ p \leftrightarrow q \iff [(\neg p \wedge \neg q) \vee (q \wedge \neg q)] \vee [(\neg p \wedge p) \vee (q \wedge p)] $$

and using identities,

$$ p \leftrightarrow q \iff [(\neg p \wedge \neg q) \vee \mathbb{0}] \vee [\mathbb{0} \vee (q \wedge p)] $$

$$ p \leftrightarrow q \iff (\neg p \wedge \neg q) \vee (q \wedge p)$$

By commution,

$$ p \leftrightarrow q \iff (p \wedge q) \vee (\neg p \wedge \neg q) $$

#### Example

Show $ \neg q \vee ( p \to q ) $ is a tautology.

##### Solution

Proof:

We know, 

$$ p \to q \iff \neg p \vee q $$

substituting,

$$ \neg q \vee ( \neg p \vee q ) $$

By commution,

$$ (\neg q \vee \neg p) \wedge ( \neg q \vee q ) $$

then using identities,

$$ (\neg q \vee \neg p) \wedge \mathbb{1} $$

and dominance,

$$ \mathbb{1} $$

__This is wrong :(__

## Section 1.3 - Logical Arguments

_definition_: an __argument__ is a type of implication, were we have many premises and one conclusion

$$ (p_1 \wedge p_2 \wedge p_3 \wedge ... \wedge p_n) \to q $$







