# Lecture 26 - Notes  

### July 7, 2015  

## Section 4.4 Continued

#### Fact

$$
    9 \equiv -1 \pmod{10}
$$

#### Example

Find the last digit of $3^{123}$.

##### Solution

We can find $3^{123} \pmod{10}$ instead

$$\begin{aligned}
    3^{123} &= 3^{120+3} \newline
    &= 3^{2 \cdot 60 + 3} \newline
    &= (3^2)^{60} \cdot 3^3 \newline
    &= 9^{60} \cdot 3^3 \newline
    &\equiv (-1)^{60} \cdot 3^3 \pmod{10} \newline
    &\equiv 27 \pmod{10} \newline
    &\equiv 7 \pmod{10} \newline
\end{aligned}$$

#### Application of Divisibility by 3

Notice if $3 \mid n$, then,

$$
    n \equiv 0 \pmod{3}
$$

also,

$$
    10 \equiv 1 \pmod{3}
$$

To test if $3 \mid n$ we will start by writing,

$$\begin{aligned}
    n &= d_k 10^k + d_{k-1} 10^{k-1} + d_{k-2} 10^{k-2} + ... + d_0 10^0 \newline
    &\equiv d_k + d_{k-1} + d_{k-2} + ... + d_0 \pmod{3} \newline
\end{aligned}$$

so

$$
    3 \mid n \iff 3 \mid \left( d_k + d_{k-1} + d_{k-2} + ... + d_0 \right)
$$

# Chapter 5 -- Induction

## Section 5.1 -- Mathematical Induction

#### Fact

The punctured $2^n \times 2^n$ chessboard can be tiled by the 3-square corner piece. Once you have the initial $2 \times 2$ board and you know the centre tile trick, you can solve any board.

#### Example

Consider a line of dominos, $1,2,3,...,n-1,n,n+1,...$ where domino $n$ falls over. This infers that dominos $n+1,n+2,...$ will fall.

We need two things to ensure all the dominos fall over,

1. We need to know one domino falls, an initial push (Basis)
2. We need to know that one domino falling will cause the others to fall (Inductive step)

### Induction

_definition_: 


#### Example

Prove that for any natural number $n \gt 1$,

$$
    \sum_{i=1}^{n} i = \frac{n(n+1)}{2}
$$

##### Solution

Let $P(n)$ be the statement,

$$
    \sum_{i=1}^{n} i = \frac{n(n+1)}{2}
$$

where $n \in \mathbb N$ and $n \gt 0$.

###### Basis

Consider the base case $P(1)$, on the left hand side,

$$\begin{aligned}
    \sum_{i=1}^{1} i &= 1
\end{aligned}$$

on the right hand side,

$$\begin{aligned}
    \frac{1 \cdot (1 + 1)}{2} &= \frac{2}{2} \newline
    &= 1 \newline
\end{aligned}$$

since the left hand side is equal to the right hand side $P(1)$ is true.

####### Inductive Hypothesis

Suppose that $P(k)$ is true for some $k \in \mathbb N$ where $k \gt 1$, i.e.,

$$\begin{aligned}
    \sum_{i=1}^{k} i = \frac{k(k+1)}{2}
\end{aligned}$$

###### Inductive Step

Consider $P(k+1)$, on the left hand side,

$$\begin{aligned}
    \sum_{i=0}^{k+1} i &= 1 + 2 + 3 + ... + k + k + 1 \newline
    &= \sum_{i=0}^{k} i + k + 1
\end{aligned}$$

by the inductive hypothesis,

$$\begin{aligned}
    \sum_{i=0}^{k+1} i &= \frac{k(k+1)}{2} + k + 1 \newline
    &= \frac{k(k+1) + 2k + 2}{2} \newline
    &= \frac{k^2 + 3k + 2}{2} \newline
    &= \frac{(k+2)(k+1)}{2} \newline
\end{aligned}$$

and if we consider the right hand side of $P(k+1)$,

$$\begin{aligned}
    \frac{(k+1)((k+1)+1)}{2} = \frac{(k+1)(k+2)}{2}.
\end{aligned}$$

The right hand side is equal to the left hand side, therefore, by induction,

$$
    \sum_{i=1}^{n} i = \frac{n(n+1)}{2}
$$

for all $n \in \mathbb N$.








